P(n) : 0 + 1 + 2 + ... n = (n(n+1) / 2)

Base case: P(0)

Inductive case: P(n) => P(n+1)

Base case:

### P(0) :

  0 + 1 + 2 + ... 0 
= 0
  by arithmetic
= (0(0+1) / 2)
  by arithmetic
Inductive case: P(n) => P(n+1)

Given: P(n) : 0 + 1 + 2 + ... n = (n(n+1) / 2)

Show: P(n+1) : 0 + 1 + 2 + ... n + n+1 = ( (n+1) (n+1 +1) / 2)

  0 + 1 + 2 + ... n + n+1 
= (0 + 1 + 2 + ... n) + n+1
  by arithmetic
= (n (n+1) /2) + n + 1
  by inductive hypothesis
= (n (n+1) /2) + (2 (n + 1) / 2)
  by arithmetic, multiplying by 2/2
= (n (n+1) /2) + ((2n + 2) / 2)
  by arithmetic
= (n (n+1)  +  (2n +2)) / 2
  by arithmetic
= (n^2 + n + 2n + 2) / 2
  by arithmetic 
= ( n^2 + 2n  + n + 2) / 2
  by aritmetic
= ( (n+1) (n+2) / 2)
  by arithmetic
= ( (n+1) (n+1 +1) / 2)