### sum
let rec sum lst = match lst with
 | [] -> 0
 | x::xs -> x + sum xs
sum (l1 @ l2) = sum l1 + sum l2

sum ([] @ l2) = sum [] + sum l2

  sum ([] @ l2) 
= sum l2
  by properties of lists and @
= 0 + sum l2
  by arithmetic
= sum [] + sum l2
  by def of sum
### Inductive case: Show sum ((x::xs) @ l2) = sum (x::xs) + sum l2 Given sum (xs @ l2) = sum xs + sum l2

  sum ((x::xs) @ l2) 
= sum ( x :: (xs @ l2) )
  by properties of lists and @
= x + sum (xs @ l2)
  by def of sum
= x + (sum xs + sum l2)
  by inductive hypothesis
= (x + sum xs) + sum l2
  by arithmetic
= sum (x::xs) + sum l2
  by def of sum
### Reverse
let rec rev lst = match lst with
  | [] -> []
  | x::xs -> rev xs @ [x]
Show rev (l1 @ l2) = rev l2 @ rev l1

Base Case: rev ([] @ l2) = rev l2 @ rev []

  rev ([] @ l2) 
= rev l2
  by properties of lists and @
= rev l2 @ []
  by properties of lists
= rev l2 @ rev []
  by def of rev
Inductive Case: 
rev ((x::xs) @ l2) = rev l2 @ rev (x::xs) Ind hyp: rev (xs @ l2) = rev l2 @ rev xs

  rev ((x::xs) @ l2) 
= rev (x :: (xs @ l2))
  by properties of lists and @
= rev (xs @ l2) @ [x]
  by def of rev
= (rev l2 @ rev xs) @ [x]
  by inductive hypothesis
= rev l2 @ (rev xs @ [x])
  by associativity of @
= rev l2 @ rev (x::xs)
  by def of rev