### Show: is_elem e (place e l)
Base case: is_elem e (place e [])
、、、
  is_elem e (place e [])
= is_elem e [e]
  by def place
= e = e || e > e && is_elem e []
  by def is_elem
= true
  for obvious reasons
、、、

### Inductive case: is_elem e (place e (y::ys)) Ind hyp.: is_elem e (place e ys)

Proof by sub-cases: e = y, e < y, e > y

Case: e = y

  is_elem e (place e (y::ys))
= is_elem e (y :: place e ys)
  by def. of place, using our assumption e = y
= e = y || (e > y && is_elem e ys)
  by def. of is_elem
= true || (e > y && is_elem e ys)
  by our assumption
= true
  by simplification
Case: e < y

  is_elem e (place e (y::ys))
= is_elem e (e::y::ys)
  by def of place
= e = e || (e > y && is_elem e ys)
  by def of is_elem
= true
  by assumption and simplification
Case: e > y

  is_elem e (place e (y::ys))
= is_elem e (y :: place e ys)
  by def of place
= e = y || (e > y && is_elem e (place e ys))
  by def of is_elem
= is_elem e (place e ys)
  by simplification and assumption of e > y
= true
  by inductive hypothesis
### Show sorted l => sorted (place e l)
Base case: sorted [] => sorted (place e [])

exercise for the reader
Ind case: sorted (y::ys) => sorted (place e (y::ys)) Ind hyp: sorted ys => sorted (place e ys)

Assume: sorted (y::ys) and then show: sorted (place e (y::ys))

Cases: e < y, e >= y, and maybe more as we see below

Case: e < y

  sorted (place e (y::ys))
= sorted (e::y::ys)
  by def of place
= e <= y && sorted (y::ys)
  by def of sorted
= true && true
  by case assumption and sorted asssumption on y::ys
Case: e >= y and ys = []

  sorted (place e (y::ys))
= sorted (y :: place e ys)
  by def of place
= sorted (y :: e :: [])
  by def of place
= y <= e && sorted (e::[])
  by def of sorted
= true && true
  by assumption and def of sorted
Case: e >= y and ys = z::zs and e < z

  sorted (place e (y::z::zs))
= sorted (y :: place e (z::zs))
  by def of place
= sorted (y :: e :: z :: zs )
  by def of place
= y <= e && sorted (e::z::zs)
  by def of sorted
= y <= e && e <= z && sorted (z::zs)
  by def of sorted
= sorted (z::zs)
  by simplification using assumptions
= true 
  by the lemma directly below
Lemma: sorted (y::z::zs) => sorted (z::zs)

  sorted (y::z::zs) => sorted (z:zs)
= (y < z && sorted (z::zs)) => sorted (z::zs)
  by def of sorted
= true
  by simplification of && and => operations
Case: e >= y and ys = z::zs and e >= z

So just one more case to solve