#Notes for November 9


let cond c t e = if c then t else e
in some use

let rec sumToN n = cond (n = 0)
                        0
                        (n + sumToN (n-1)
Ease of expression using lazy evaluation.
using lazy evaluation
```
  eqleaves_v1 (Lf (3 * 3)) (Nd (Lf (3 + 3), Lf (2 * 5)))

= equal_list (flatten (Lf (3 * 3))) (flatten (Nd (Lf (3 + 3), Lf (2 *
5))))

= equal_list [3 * 3] (flatten (Nd (Lf (3 + 3), Lf (2 * 5))))

= equal_list [3 * 3] (append (flatten (Lf (3 + 3))) (flatten (Lf (2 *
5))))

= equal_list [3 * 3] (append [3 + 3] (flatten (Lf (2 * 5))))

= equal_list [3 * 3] (3 + 3 :: append [] (flatten (Lf (2 * 5))))

= if (3 * 3) = (3 + 3)

  then equal_list [] (append [] flatten (Lf (2 * 5))) 

  else false

= if 9 = (3 + 3)

  then equal_list [] (append [] flatten (Lf (2 * 5))) 

  else false

= if 9 = 6

  then equal_list [] (append [] flatten (Lf (2 * 5))) 

  else false

= if false

  then equal_list [] (append [] flatten (Lf (2 * 5))) 

  else false

= false
Version 1 - eagerly and slow

  eqleaves_v1 (Lf (3 * 3)) (Nd (Lf (3 + 3), Lf (2 * 5)))

= eqleaves_v1 (Lf 9) (Nd (Lf 6, Lf 10))

= equal_list (flatten (Lf 9)) (flatten (Nd (Lf 6, Lf 10)))

= equal_list [9] (flatten (Nd (Lf 6, Lf 10)))

= equal_list [9] (append (flatten (Lf 6)) (flatten (Lf 10)))

= equal_list [9] (append [6] (flatten (Lf 10)))

= equal_list [9] (6 :: append [] (flatten (Lf 10)))

= equal_list [9] (6 :: (flatten (Lf 10)))

= equal_list [9] (6 :: [10])

= equal_list [9] [6; 10]

= if 9 = 6 then equal_list [] [10] else false

= false
Version 2 - eagerly and fast

  eqleaves_v2 (Lf (3 * 3)) (Nd (Lf (3 + 3), Lf (2 * 5)))

= eqleaves_v2 (Lf 9) (Nd (Lf 6, Lf 10))

= comparestacks [Lf 9] [Nd (Lf 6, Lf 10)]

= comparestacks [Lf 9] [Lf 6; Lf 10]

= if 9 = 6 then comparestacks [] [Lf 10] else false

= false
Exercise 4.1 #4
sum (take 2 (squares_from 3))

sum (take 2 ( 3*3 :: squares_from (3+1) )

sum ( (3*3) :: take (2-1) (squares_from (3+1)) )

(3*3) + (sum (take (2-1) (squares_from (3+1))))

9 + (sum (take (2-1) (squares_from (3+1))))

9 + (sum (take 1 (squares_from (3+1))))

9 + (sum (take 1 ( (a1 * a1) :: squares_from (a1 + 1))))
  where a1 = 3+1

9 + (sum ( (a1 * a1) :: (take (1-1) ( squares_from (a1 + 1)))))
  where a1 = 3+1 

9 + ((a1 * a1) + ( sum (take (1-1) ( squares_from (a1 + 1)))))
  where a1 = 3+1 

9 + ((a1 * a1) + ( sum (take (1-1) ( squares_from (a1 + 1)))))
  where a1 = 4

9 + ((4 * 4) + ( sum (take (1-1) ( squares_from (4 + 1)))))

9 + (16 + ( sum (take 0 ( squares_from (4 + 1)))))

9 + (16 + ( sum [] ) )

9 + (16 + ( 0 ) )

9 + 16

25
```